rename frameclass

Foundation/Modal/Kripke/Logic/K45.lean
@@ -12,7 +12,7 @@ namespace Kripke
 
 protected class Frame.IsK45 (F : Kripke.Frame) extends F.IsTransitive, F.IsEuclidean
 
-protected abbrev FrameClass.IsK45 : FrameClass := { F | F.IsK45 }
+protected abbrev FrameClass.K45 : FrameClass := { F | F.IsK45 }
 
 instance {F : Kripke.Frame} [F.IsK45] : F.IsK4Point3 where
 
@@ -21,22 +21,22 @@ end Kripke
 
 namespace Logic.K45.Kripke
 
-instance : Sound Hilbert.K45 FrameClass.IsK45 := instSound_of_validates_axioms $ by
+instance : Sound Hilbert.K45 FrameClass.K45 := instSound_of_validates_axioms $ by
   apply FrameClass.Validates.withAxiomK;
   rintro F ⟨_, _⟩ _ (rfl | rfl);
   . exact validate_AxiomFour_of_transitive;
   . exact validate_AxiomFive_of_euclidean;
 
-instance : Entailment.Consistent Hilbert.K45 := consistent_of_sound_frameclass FrameClass.IsK45 $ by
+instance : Entailment.Consistent Hilbert.K45 := consistent_of_sound_frameclass FrameClass.K45 $ by
   use whitepoint;
   constructor;
 
 
-instance : Canonical Hilbert.K45 FrameClass.IsK45 := ⟨by constructor⟩
+instance : Canonical Hilbert.K45 FrameClass.K45 := ⟨by constructor⟩
 
-instance : Complete Hilbert.K45 FrameClass.IsK45 := inferInstance
+instance : Complete Hilbert.K45 FrameClass.K45 := inferInstance
 
-lemma trans_eucl : Modal.K45 = FrameClass.IsK45.logic := eq_hilbert_logic_frameClass_logic
+lemma trans_eucl : Modal.K45 = FrameClass.K45.logic := eq_hilbert_logic_frameClass_logic
 
 instance : Hilbert.K5 ⪱ Hilbert.K45 := by
   constructor;
@@ -60,7 +60,7 @@ instance : Hilbert.K5 ⪱ Hilbert.K45 := by
 
 instance : Hilbert.K4Point3 ⪱ Hilbert.K45 := by
   constructor;
-  . apply Hilbert.Kripke.weakerThan_of_subset_frameClass FrameClass.IsK4Point3 FrameClass.IsK45;
+  . apply Hilbert.Kripke.weakerThan_of_subset_frameClass FrameClass.K4Point3 FrameClass.K45;
     intro F hF;
     simp_all only [Set.mem_setOf_eq];
     infer_instance;
@@ -68,7 +68,7 @@ instance : Hilbert.K4Point3 ⪱ Hilbert.K45 := by
     use (Axioms.Five (.atom 0));
     constructor;
     . simp;
-    . apply Sound.not_provable_of_countermodel (𝓜 := FrameClass.IsK4Point3);
+    . apply Sound.not_provable_of_countermodel (𝓜 := FrameClass.K4Point3);
       apply Kripke.not_validOnFrameClass_of_exists_model_world;
       let M : Model := ⟨
         ⟨Fin 3, λ x y => x < y⟩,
